bin/templates/dafny_skeleton.dfy
@@ -1,79 +1,58 @@
-/***************************** UTIL Functions *******************************/
-function str_equal(val1: int, val2: int) : bool
-{
-  val1 == val2
-}
+/***************************** INCLUDES *************************************/
+include "utils.dfy"
 
 /***************************** DO MAP ***************************************/
+
 <emit-funcs>
 function domap (<mapper-args-decl>) : <domap-emit-type>
-  <loop-counter-range-domap>
-  ensures domap(<mapper-args-call>) == <domap-emits>
+    <emit-requires>
+    ensures domap(<mapper-args-call>) == <domap-emits>
 {
-  <domap-emits>
+    <domap-emits>
 }
 
 /***************************** MAPPER ***************************************/
 
 function mapper (<mapper-args-decl>) : <domap-emit-type>
-  <loop-counter-range-map>
+    <mapper-requires>
 {
-  if <terminate-condition> then []
-  else domap(<mapper-args-call-inductive>) + mapper(<mapper-args-call-inductive>)
+    if <terminate-condition> then []
+    else domap(<mapper-args-call-inductive>) + mapper(<mapper-args-call-inductive>)
 }
 
 /***************************** DO REDUCE ************************************/
 
 function doreduce(input: <domap-emit-type>, key: <doreduce-key-type><reducer-args-decl>) : <output-type>
-  ensures (|input| > 0 && input[0].0 == key) ==> 
-      doreduce(input, key<reducer-args-call>) == (<reduce-exp>)
-  ensures (|input| > 0 && input[0].0 != key) ==> 
-      doreduce(input, key<reducer-args-call>) == doreduce(input[1..], key<reducer-args-call>)
+    ensures (|input| > 0 && input[0].0 == key) ==> 
+        doreduce(input, key<reducer-args-call>) == (<reduce-exp>)
+    ensures (|input| > 0 && input[0].0 != key) ==> 
+        doreduce(input, key<reducer-args-call>) == doreduce(input[1..], key<reducer-args-call>)
 {
-  if input == [] then <reduce-init-value> 
-  else if input[0].0 == key then (<reduce-exp>)
-  else doreduce(input[1..], key<reducer-args-call>)
+    if input == [] then (<reduce-init-value> )
+    else if input[0].0 == key then (<reduce-exp>)
+    else doreduce(input[1..], key<reducer-args-call>)
 }
 
-/******************************* HARNESS ************************************/  
-
-function contains(input: <domap-emit-type>, key: <doreduce-key-type>) : bool
-  ensures (input == []) ==> (contains(input, key) == false)
-  ensures (|input| > 0 && input[0].0 == key) ==> (contains(input, key) == true)
-  ensures (|input| > 0 && input[0].0 != key) ==> (contains(input, key) == contains(input[1..], key))
-{
-  if input == [] then false
-  else if input[0].0 == key then true
-  else contains(input[1..], key)
-}
+/******************************* HARNESS ************************************/    
 
 <reduce-exp-lemma>
-
-lemma Lemma (<inv-pc-args>)
-  <lemma-requires>
-  requires <invariant>
-  
-{
-  assert mapper(<mapper-args-call-inductive-2>) == domap(<mapper-args-call>) + mapper(<mapper-args-call>);
-
-  <emit-lemmas>
-}
+<conditional-lemma>
 
 predicate loopInvariant (<inv-pc-args>)
-  <inv-requires>
+    <inv-requires>
 {
-  <loop-inv>
+    <loop-inv>
 }
 
 predicate postCondition (<inv-pc-args>)
-  <pcond-requires>
+    <inv-requires>
 {
-  <post-cond>
+    <post-cond>
 }
 
 method harness (<harness-args>)
-  <main-requires>
+    <main-requires>
 {
-  <init-vars>
-  <verif-code>
+    <init-vars>
+    <verif-code>
 }
