bin/test.sh
@@ -1,12 +1,12 @@
-./compileAndRun.sh benchmarks/Sum.java sum.java
-./run.sh benchmarks/Count.java count.java
-./run.sh benchmarks/ConditionalCount.java condcount.java
-./run.sh benchmarks/ConditionalSum.java condsum.java
-./run.sh benchmarks/Average.java avg.java
-./run.sh benchmarks/Equal.java eq.java
-./run.sh benchmarks/EqualFrequency.java eqfre.java
-./run.sh benchmarks/Histogram.java hist.java
-./run.sh benchmarks/WordCount.java wordCount.java
-./run.sh benchmarks/StatsUtilList.java stl.java
-./run.sh benchmarks/LinearRegression.java lr.java
+./compileAndRun.sh benchmarks/Sum.java sum.java &&
+./run.sh benchmarks/Count.java count.java &&
+./run.sh benchmarks/ConditionalCount.java condcount.java &&
+./run.sh benchmarks/ConditionalSum.java condsum.java &&
+./run.sh benchmarks/Average.java avg.java &&
+./run.sh benchmarks/Equal.java eq.java &&
+./run.sh benchmarks/EqualFrequency.java eqfre.java &&
+./run.sh benchmarks/Histogram.java hist.java &&
+./run.sh benchmarks/WordCount.java wordCount.java &&
+./run.sh benchmarks/StatsUtilList.java stl.java &&
+./run.sh benchmarks/LinearRegression.java lr.java &&
 ./run.sh benchmarks/StringMatch.java strMatch.java
